src/Lib/DWT/VST/Ber_tlv_length_serialize.v
@@ -39,7 +39,9 @@ Definition der_tlv_length_serialize_spec : ident * funspec :=
 
 Definition Gprog := ltac:(with_library prog [der_tlv_length_serialize_spec]).
 
-(* Theorem ber_tlv_length_serialize_correct' : 
+(*
+
+Theorem ber_tlv_length_serialize_correct' : 
   semax_body Vprog Gprog (normalize_function f_der_tlv_length_serialize composites)
              der_tlv_length_serialize_spec.
 Proof.
